src/Generated/AwsCryptographicMaterialProviders.dfy
@@ -77,7 +77,7 @@ module {:extern "Dafny.Aws.Crypto"} Aws.Crypto {
             true
         }
     }
-
+    
     datatype DecryptionMaterials = DecryptionMaterials(nameonly algorithmSuiteId: AlgorithmSuiteId,
                                                        nameonly encryptionContext: EncryptionContext,
                                                        nameonly plaintextDataKey: Option<seq<uint8>>,
@@ -322,7 +322,7 @@ module {:extern "Dafny.Aws.Crypto"} Aws.Crypto {
         // method CreateMrkAwareDiscoveryMultiKeyring(input: CreateMrkAwareDiscoveryMultiKeyringInput) returns (res: IKeyring)
         method CreateMultiKeyring(input: CreateMultiKeyringInput) returns (res: IKeyring?)
         method CreateRawAesKeyring(input: CreateRawAesKeyringInput) returns (res: IKeyring)
-        method CreateRawRsaKeyring(input: CreateRawRsaKeyringInput) returns (res: IKeyring)
+        method CreateRawRsaKeyring(input: CreateRawRsaKeyringInput) returns (res: Result<IKeyring, string>)
 
         // CMMs
         method CreateDefaultCryptographicMaterialsManager(input: CreateDefaultCryptographicMaterialsManagerInput) returns (res: ICryptographicMaterialsManager)
